syntactic causality

Coq/Causality.v
@@ -7,20 +7,20 @@ Open Scope Z.
 
 (* [obs_until d r1 r2] iff [r1] [r2] coincide at [d] and earlier. *)
 
-Definition ext_until (d : Z) (r1 r2 : ext) : Prop :=
-  forall z, Z.le z d -> r1 z = r2 z.
+Definition ext_until (d : Z) (r1 r2 : ExtEnv) : Prop :=
+  forall l z, Z.le z d -> r1 l z = r2 l z.
 
 (* Semantic causality *)
 
-Definition causal (c : contract) : Prop :=
+Definition causal (c : Contr) : Prop :=
   forall d r1 r2,  ext_until (Z.of_nat d) r1 r2 -> (C[|c|]r1) d = (C[|c|]r2) d.
 
 
-Lemma ext_until_adv d t (r1 r2 : ext): 
+Lemma ext_until_adv d t (r1 r2 : ExtEnv): 
   ext_until d (adv_ext t r1) (adv_ext t r2) <-> ext_until (t + d) r1 r2.
 Proof.
   unfold ext_until,adv_ext. split; intros.
-  - pose (H (z - t)%Z). 
+  - pose (H l (z - t)%Z). 
     assert (t + (z - t) = z)%Z as E. omega. rewrite E in *. 
     apply e. omega.
   - apply H. omega.
@@ -35,7 +35,7 @@ Proof.
   rewrite ext_until_adv. rewrite H1. assumption.
 Qed.
 
-Lemma ext_until_le d1 d2 (r1 r2 : ext) : ext_until d1 r1 r2 ->  d2 <= d1 -> ext_until d2 r1 r2.
+Lemma ext_until_le d1 d2 (r1 r2 : ExtEnv) : ext_until d1 r1 r2 ->  d2 <= d1 -> ext_until d2 r1 r2.
 Proof. 
   unfold ext_until. intros. apply H. omega.
 Qed.
